fun-op-sem: improved file structure, more comments

examples/fun-op-sem/for/for_nd_compileScript.sml
@@ -1,9 +1,23 @@
 open HolKernel Parse boolLib bossLib;
 
-val _ = new_theory "lang_compile";
+val _ = new_theory "for_nd_compile";
+
+(*
+
+This file proves correctness of a compiler for the FOR language
+defined in for_ndScript.sml and for_nd_semScript.sml. The compiler
+targets a simple assembly-like language. We prove that the compiler
+preserves the top-level observable semantics.
+
+The compiler consists of three passes:
+ - the first pass simplifies For loops and removes Dec
+ - the second pass compiles expressions into very simple assignments
+ - the third pass maps the FOR language into assmembly code
+
+*)
 
 open optionTheory pairTheory pred_setTheory finite_mapTheory stringTheory;
-open lcsymtacs langTheory funTheory listTheory arithmeticTheory;
+open lcsymtacs for_ndTheory for_nd_semTheory listTheory arithmeticTheory;
 
 val _ = temp_tight_equality ();
 
@@ -11,7 +25,21 @@ val ect = BasicProvers.EVERY_CASE_TAC;
 
 val IMP_IMP = METIS_PROVE [] ``b /\ (b1 ==> b2) ==> ((b ==> b1) ==> b2)``
 
-(* verification of PASS 1, which reduces complexity of For and removes Dec *)
+
+(* === PASS 1 : simplifies For loops and removes Dec === *)
+
+val Loop_def = Define `
+  Loop t = For (Num 1) (Num 1) t`;
+
+val pass1_def = Define `
+  (pass1 (Exp e) = Exp e) /\
+  (pass1 (Dec x t) = Seq (Exp (Assign x (Num 0))) (pass1 t)) /\
+  (pass1 (Break) = Break) /\
+  (pass1 (Seq t1 t2) = Seq (pass1 t1) (pass1 t2)) /\
+  (pass1 (If e t1 t2) = If e (pass1 t1) (pass1 t2)) /\
+  (pass1 (For e1 e2 t) = Loop (If e1 (Seq (pass1 t) (Exp e2)) Break))`;
+
+(* Verification of pass 1 *)
 
 val sem_t_Dec = store_thm("sem_t_Dec",
   ``sem_t s (Dec v t) =
@@ -26,9 +54,6 @@ val sem_t_pull_if = prove(
 val sem_t_eval = save_thm("sem_t_eval",
   (EVAL THENC REWRITE_CONV [sem_t_pull_if] THENC EVAL)
     ``sem_t s (If b (Exp (Num 0)) Break)``);
-
-val Loop_def = Define `
-  Loop t = For (Num 1) (Num 1) t`;
 
 val sem_t_Loop = save_thm("sem_t_Loop",
   ``sem_t s (Loop t)``
@@ -77,14 +102,6 @@ val sem_t_For = store_thm("sem_t_For",
   \\ imp_res_tac sem_t_clock
   \\ decide_tac);
 
-val pass1_def = Define `
-  (pass1 (Exp e) = Exp e) /\
-  (pass1 (Dec x t) = Seq (Exp (Assign x (Num 0))) (pass1 t)) /\
-  (pass1 (Break) = Break) /\
-  (pass1 (Seq t1 t2) = Seq (pass1 t1) (pass1 t2)) /\
-  (pass1 (If e t1 t2) = If e (pass1 t1) (pass1 t2)) /\
-  (pass1 (For e1 e2 t) = Loop (If e1 (Seq (pass1 t) (Exp e2)) Break))`;
-
 val pass1_correct = store_thm("pass1_correct",
   ``!t s. sem_t s (pass1 t) = sem_t s t``,
   Induct \\ fs [pass1_def,sem_t_def_with_stop,GSYM sem_t_For,GSYM sem_t_Dec]
@@ -97,7 +114,7 @@ val pass1_pres = store_thm("pass1_pres",
   \\ fs [semantics_def,pass1_correct]);
 
 
-(* verification of PASS 2, which flattens all expressions *)
+(* === PASS 2 : compiles expressions into very simple assignments === *)
 
 val comp_exp_def = Define `
   (comp_exp (Var v) s = Exp (Assign s (Var v))) /\
@@ -140,6 +157,8 @@ val t_max_def = Define `
 
 val pass2_def = Define `
   pass2 t = flatten_t t ("temp" ++ REPLICATE (t_max t - 3) #"'")`;
+
+(* Verification of pass 2 *)
 
 val possible_var_name_def = Define `
   possible_var_name v s = !n. ~(v ++ REPLICATE n #"'" IN FDOM s)`;
@@ -430,6 +449,12 @@ val lemma = prove(
   ``((if b then x1 else x2) <> x2) <=> (x1 <> x2) /\ b``,
   Cases_on `b` \\ fs [])
 
+(* We prove that pass 2 preserves semantics: any behaviour that the
+   generated code has must also be behaviour of the input program, if
+   the source semantics does not contain Crash (implied by successful
+   type check) and if the syntax of the compiler program fits with
+   pass2_subset (i.e. syntax produced by pass1) *)
+
 val pass2_pres = store_thm("pass2_pres",
   ``!t input. ~(Crash IN semantics t input) /\ pass2_subset t ==>
               semantics (pass2 t) input SUBSET semantics t input``,
@@ -471,7 +496,9 @@ val pass2_pres = store_thm("pass2_pres",
   \\ METIS_TAC []);
 
 
-(* verification of PASS 3, which generates assmebly programs *)
+(* === PASS 3 : maps the FOR language into assmembly code === *)
+
+(* We define the tagert deterministic assembly language *)
 
 val _ = Datatype `
 reg = Reg string`
@@ -572,28 +599,32 @@ val a_state_def = Define `
 
 val asm_semantics_def = Define `
 (asm_semantics code input (Terminate io_trace) =
-  (* Terminate when there is a clock and some non-determinism oracle that gives a value result *)
+  (* Terminate when there is a clock and some non-determinism oracle
+     that gives a value result *)
   ?c i s.
     sem_a (a_state code c input) = (Rval i, s) /\
     s.state.io_trace = io_trace) /\
 (asm_semantics code input Crash =
-  (* Crash when there is a clock that gives a non-value, non-timeout result *)
+  (* Crash when there is a clock that gives a non-value, non-timeout
+     result *)
   ?c r s.
     sem_a (a_state code c input) = (r, s) /\
     (r = Rbreak \/ r = Rfail)) /\
 (asm_semantics code input (Diverge io_trace) <=>
-  (* Diverge when all clocks give timeout results. Ensure that the IO trace to
-   * the timeout point is a prefix of the whole trace. *)
+  (* Diverge when all clocks give timeout results. Ensure that the IO
+     trace to the timeout point is a prefix of the whole trace. *)
     (!c. ?s.
       sem_a (a_state code c input) = (Rtimeout, s) /\
       (!n. n < LENGTH s.state.io_trace ==>
            LNTH n io_trace = SOME (EL n s.state.io_trace))) /\
-    (* Check that the whole IO trace is reachable, but maybe not for just 1
-     * clock value*)
+    (* Check that the whole IO trace is reachable, but maybe not for
+       just 1 clock value *)
     (!n x.
       LNTH n io_trace = SOME x ==>
       ?c s. sem_a (a_state code c input) = (Rtimeout, s) /\
             n < LENGTH s.state.io_trace /\ EL n s.state.io_trace = x))`;
+
+(* Definition of pass3 *)
 
 val pass3_aux_def = Define `
   (pass3_aux n (Dec v t) b = []) /\
@@ -624,6 +655,8 @@ val pass3_aux_def = Define `
 
 val pass3_def = Define `
   pass3 t = pass3_aux 0 t 0 ++ [Halt]`;
+
+(* Verification of pass3 *)
 
 val LENGTH_pass3_aux = prove(
   ``!t n b. LENGTH (pass3_aux n t b) = LENGTH (pass3_aux 0 t 0)``,
@@ -923,6 +956,10 @@ val pass3_correct = store_thm("pass3_correct",
   \\ SIMP_TAC std_ss [Once sem_a_def]
   \\ fs [rich_listTheory.EL_LENGTH_APPEND]);
 
+(* We prove that pass3 preserves semantics if the source does not
+   contain Crash and if the syntax fits within the subset defined by
+   pass3_subset. *)
+
 val pass3_pres = store_thm("pass3_pres",
   ``!t input. ~(Crash IN semantics t input) /\ pass3_subset t ==>
               asm_semantics (pass3 t) input SUBSET semantics t input``,
@@ -968,10 +1005,13 @@ val pass3_pres = store_thm("pass3_pres",
   \\ fs [s_with_clock_def,init_st_def,a_state_def]
   \\ Q.LIST_EXISTS_TAC [`c`] \\ fs []);
 
-(* the entire compiler *)
+
+(* === The end-to-end compiler === *)
 
 val compile_def = Define `
   compile t = pass3 (pass2 (pass1 t))`;
+
+(* Verification of the compile function *)
 
 val pass2_subset_pass1 = prove(
   ``!t. pass2_subset (pass1 t)``,
@@ -992,6 +1032,10 @@ val pass3_subset_pass2_pass1 = prove(
   \\ MATCH_MP_TAC pass3_subset_flatten_t
   \\ fs [pass2_subset_pass1]);
 
+(* Any observable behaviour of the compiled code is also observable
+   behaviour of the source code, if Crash is not an observable
+   behaviour of the course program. *)
+
 val compile_pres = store_thm("compile_pres",
   ``!t input. ~(Crash IN semantics t input) ==>
         asm_semantics (compile t) input SUBSET semantics t input``,
@@ -1009,12 +1053,16 @@ val compile_pres = store_thm("compile_pres",
     \\ METIS_TAC [])
   \\ MATCH_MP_TAC pass2_pres \\ fs [pass2_subset_pass1]);
 
+(* The simple type checker (defined in for_nd_semScript.sml) ensures
+   that the source program cannot Crash. This leads to a cleaner
+   top-level correctness theorem for compile. *)
+
 val syntax_ok_def = Define `
-  syntax_ok t = !input. ~(Crash IN semantics t input)`;
+  syntax_ok t = type_t F {} t`;
 
 val compile_correct = store_thm("compile_correct",
-  ``!t i. syntax_ok t ==>
-          asm_semantics (compile t) i SUBSET semantics t i``,
-  METIS_TAC [syntax_ok_def,compile_pres]);
+  ``!t inp. syntax_ok t ==>
+            asm_semantics (compile t) inp SUBSET semantics t inp``,
+  METIS_TAC [type_soundness,syntax_ok_def,compile_pres]);
 
 val _ = export_theory ();
