examples/fun-op-sem/for/for_nd_semScript.sml
@@ -1,20 +1,30 @@
 open HolKernel Parse boolLib bossLib;
 
-val _ = new_theory "fun";
+val _ = new_theory "for_nd_sem";
+
+(*
+
+This file defines a functional big-step semantics for the FOR language
+syntax given in for_ndScript.sml. The language has basic I/O and
+non-deterministic evaluation order.
+
+A simpler version of this language can be found in forScript.sml.
+
+*)
 
 open optionTheory pairTheory pred_setTheory finite_mapTheory stringTheory;
 open llistTheory integerTheory;
-open langTheory;
+open for_ndTheory;
 open lcsymtacs;
 
 val ect = BasicProvers.EVERY_CASE_TAC;
 
 val _ = temp_tight_equality ();
 
-(* The result of running a program. Rtimeout indicates an attempt to loop with
- * no clock left. Rfail indicates an undeclared variable access or a Break not
- * in a For.
- *)
+(* The result of running a program. Rtimeout indicates an attempt to
+   loop with no clock left. Rfail indicates an undeclared variable
+   access or a Break not in a For. *)
+
 val _ = Datatype `
 r = Rval int
   | Rbreak
@@ -29,10 +39,10 @@ val _ = type_abbrev ("oracle", ``:(num -> 'a)``);
 val oracle_get_def = Define `
 oracle_get (f:'a oracle) = (f 0, f o ((+) 1))`;
 
-(* The state of the semantics.
- * io_trace records all IO done. input is the input stream, and non_det_o is an
- * oracle used to decide which subexpression of Add to evaluate first.
- *)
+(* The state of the semantics. Here io_trace records all I/O that has
+   been done, input is the input stream, and non_det_o is an oracle
+   used to decide which subexpression of Add to evaluate first. *)
+
 val _ = Datatype `
 state = <| store : string |-> int; clock : num; io_trace : io_tag list;
            input : char llist; non_det_o : bool oracle |>`;
@@ -56,6 +66,8 @@ unpermute_pair (x,y) switch =
     (y,x)
   else
     (x,y)`;
+
+(* Expression evaluation *)
 
 val sem_e_def = tDefine "sem_e" `
 (sem_e s (Var x) =
@@ -95,46 +107,33 @@ val sem_e_def = tDefine "sem_e" `
 
 val sem_e_ind = fetch "-" "sem_e_ind";
 
+(* HOL4's definition requires a little help with the definition. In
+   particular, we need to help it see that the clock does not
+   decrease. To do this, we add a few redundant checks (check_clock)
+   to the definition of the sem_t function. These redundant checks are
+   removed later in the script. *)
+
 val sem_e_clock = Q.store_thm ("sem_e_clock",
 `!s e r s'. sem_e s e = (r, s') ⇒ s.clock = s'.clock`,
- ho_match_mp_tac sem_e_ind >>
- rw [sem_e_def] >>
- ect >>
+ ho_match_mp_tac sem_e_ind >> rw [sem_e_def] >> ect >>
  fs [LET_THM, permute_pair_def, oracle_get_def, unpermute_pair_def, getchar_def] >>
- rw [] >>
- ect >>
- fs [] >>
- ect >>
- fs [] >>
- rw []);
+ rw [] >> ect >> fs [] >>
+ ect >> fs [] >> rw []);
 
 val sem_e_store = Q.prove (
 `!s e r s'. sem_e s e = (r, s') ⇒ FDOM s.store ⊆ FDOM s'.store`,
- ho_match_mp_tac sem_e_ind >>
- rw [sem_e_def] >>
- ect >>
- fs [SUBSET_DEF, LET_THM, permute_pair_def, oracle_get_def, unpermute_pair_def, getchar_def] >>
- rw [] >>
- ect >>
- fs [] >>
- ect >>
- fs [] >>
- rw [] >>
- metis_tac []);
+ ho_match_mp_tac sem_e_ind >> rw [sem_e_def] >> ect >>
+ fs [SUBSET_DEF, LET_THM, permute_pair_def, oracle_get_def,
+     unpermute_pair_def, getchar_def] >>
+ rw [] >> ect >> fs [] >>
+ ect >> fs [] >> rw [] >> metis_tac []);
 
 val sem_e_res = Q.store_thm ("sem_e_res",
 `!s e r s'. sem_e s e = (r, s') ⇒ r ≠ Rbreak ∧ r ≠ Rtimeout`,
- ho_match_mp_tac sem_e_ind >>
- rw [sem_e_def] >>
- ect >>
+ ho_match_mp_tac sem_e_ind >> rw [sem_e_def] >> ect >>
  fs [LET_THM, permute_pair_def, oracle_get_def, unpermute_pair_def, getchar_def] >>
- rw [] >>
- ect >>
- fs [] >>
- ect >>
- fs [] >>
- rw [] >>
- metis_tac []);
+ rw [] >> ect >> fs [] >>
+ ect >> fs [] >> rw [] >> metis_tac []);
 
 val check_clock_def = Define `
 check_clock s' s =
@@ -146,6 +145,8 @@ dec_clock s = s with clock := s.clock - 1`;
 val dec_clock_store = Q.store_thm ("dec_clock_store[simp]",
 `!s. (dec_clock s).store = s.store`,
  rw [dec_clock_def]);
+
+(* Statement evaluation -- with redundant check_clock *)
 
 val sem_t_def = tDefine "sem_t" `
 (sem_t s (Exp e) = sem_e s e) ∧
@@ -195,17 +196,11 @@ val sem_t_def = tDefine "sem_t" `
 val sem_t_clock = Q.store_thm ("sem_t_clock",
 `!s t r s'. sem_t s t = (r, s') ⇒ s'.clock ≤ s.clock`,
  ho_match_mp_tac (fetch "-" "sem_t_ind") >>
- reverse (rpt strip_tac) >>
- pop_assum mp_tac >>
- rw [Once sem_t_def] >>
- ect >>
- imp_res_tac sem_e_clock >>
- fs [] >>
+ reverse (rpt strip_tac) >> pop_assum mp_tac >>
+ rw [Once sem_t_def] >> ect >>
+ imp_res_tac sem_e_clock >> fs [] >>
  fs [check_clock_def, dec_clock_def, LET_THM] >>
- TRY decide_tac >>
- rfs [] >>
- res_tac >>
- decide_tac);
+ TRY decide_tac >> rfs [] >> res_tac >> decide_tac);
 
 val check_clock_id = Q.store_thm ("check_clock_id",
 `!s s'. s.clock ≤ s'.clock ⇒ check_clock s s' = s`,
@@ -213,6 +208,8 @@ val check_clock_id = Q.store_thm ("check_clock_id",
 
 val STOP_def = Define `
   STOP x = x`;
+
+(* Statement evaluation -- with redundant check_clock *)
 
 val sem_t_def_with_stop = Q.store_thm ("sem_t_def_with_stop",
 `(sem_t s (Exp e) = sem_e s e) ∧
@@ -250,21 +247,19 @@ val sem_t_def_with_stop = Q.store_thm ("sem_t_def_with_stop",
                    (Rval 0, s2)
                | r => r)
       | r => r)`,
- rpt strip_tac >>
- rw [Once sem_t_def,STOP_def] >>
- ect >>
- fs [] >>
+ rpt strip_tac >> rw [Once sem_t_def,STOP_def] >> ect >> fs [] >>
  imp_res_tac sem_t_clock >>
  fs [dec_clock_def, LET_THM, check_clock_id] >>
  rpt (AP_TERM_TAC ORELSE AP_THM_TAC) >>
  rw [state_component_equality] >>
  rw [check_clock_def] >>
  imp_res_tac sem_e_clock >>
- fs [] >>
- `F` by decide_tac);
+ fs [] >> `F` by decide_tac);
 
 val sem_t_def =
   save_thm("sem_t_def",REWRITE_RULE [STOP_def] sem_t_def_with_stop);
+
+(* We also remove the redundant checks from the induction theorem. *)
 
 val sem_t_ind = Q.store_thm ("sem_t_ind",
 `∀P.
@@ -294,17 +289,53 @@ val sem_t_ind = Q.store_thm ("sem_t_ind",
         P s (For e1 e2 t)) ⇒
      ∀v v1. P v v1`,
  ntac 2 strip_tac >>
- ho_match_mp_tac (fetch "-" "sem_t_ind") >>
- rw [] >>
+ ho_match_mp_tac (fetch "-" "sem_t_ind") >> rw [] >>
  first_x_assum match_mp_tac >>
- rw [] >>
- fs [] >>
- res_tac >>
+ rw [] >> fs [] >> res_tac >>
  imp_res_tac sem_t_clock >>
  imp_res_tac sem_e_clock >>
  fs [dec_clock_def, check_clock_id, LET_THM] >>
  first_x_assum match_mp_tac >>
  decide_tac);
+
+(* The top-level semantics defines what is externally observable. *)
+
+val init_st_def = Define `
+init_st c nd i =
+  <| store := FEMPTY; clock := c; input := i; io_trace := []; non_det_o := nd |>`;
+
+(* There can be many observable behaviours because the semantics is
+   non-deterministic. *)
+
+val semantics_def = Define `
+(semantics t input (Terminate io_trace) =
+  (* Terminate when there is a clock and some non-determinism oracle
+     that gives a value result *)
+  ?c nd i s.
+    sem_t (init_st c nd input) t = (Rval i, s) ∧
+    s.io_trace = io_trace) ∧
+(semantics t input Crash =
+  (* Crash when there is a clock that gives a non-value, non-timeout
+     result. *)
+  ?c nd r s.
+    sem_t (init_st c nd input) t = (r, s) ∧
+    (r = Rbreak ∨ r = Rfail)) ∧
+(semantics t input (Diverge io_trace) =
+  (* Diverge when all clocks give timeout results. Ensure that the IO
+     trace to the timeout point is a prefix of the whole trace. *)
+  ?nd.
+    (!c. ?s.
+      sem_t (init_st c nd input) t = (Rtimeout, s) ∧
+      (!n. n < LENGTH s.io_trace ⇒ LNTH n io_trace = SOME (EL n s.io_trace))) ∧
+    (* Check that the whole IO trace is reachable, but maybe not for
+       just 1 clock value *)
+    (!n x.
+      LNTH n io_trace = SOME x ⇒
+      ?c s. sem_t (init_st c nd input) t = (Rtimeout, s) ∧
+            n < LENGTH s.io_trace ∧ EL n s.io_trace = x))`;
+
+
+(* === Misc lemmas === *)
 
 val sem_t_store = Q.prove (
 `!s t r s'. sem_t s t = (r, s') ⇒ FDOM s.store ⊆ FDOM s'.store`,
@@ -364,41 +395,8 @@ val sem_for_not_break = Q.store_thm ("sem_for_not_break",
  imp_res_tac sem_e_res >>
  fs []);
 
-(* Define a top-level semantic function that maps programs and their input to
- * their observable behaviours.
- *)
-val init_st_def = Define `
-init_st c nd i =
-  <| store := FEMPTY; clock := c; input := i; io_trace := []; non_det_o := nd |>`;
 
-(* There can be many observable behaviours because the semantics is
- * non-deterministic *)
-val semantics_def = Define `
-(semantics t input (Terminate io_trace) =
-  (* Terminate when there is a clock and some non-determinism oracle that gives a value result *)
-  ?c nd i s.
-    sem_t (init_st c nd input) t = (Rval i, s) ∧
-    s.io_trace = io_trace) ∧
-(semantics t input Crash =
-  (* Crash when there is a clock that gives a non-value, non-timeout result *)
-  ?c nd r s.
-    sem_t (init_st c nd input) t = (r, s) ∧
-    (r = Rbreak ∨ r = Rfail)) ∧
-(semantics t input (Diverge io_trace) =
-  (* Diverge when all clocks give timeout results. Ensure that the IO trace to
-   * the timeout point is a prefix of the whole trace. *)
-  ?nd.
-    (!c. ?s.
-      sem_t (init_st c nd input) t = (Rtimeout, s) ∧
-      (!n. n < LENGTH s.io_trace ⇒ LNTH n io_trace = SOME (EL n s.io_trace))) ∧
-    (* Check that the whole IO trace is reachable, but maybe not for just 1
-     * clock value*)
-    (!n x.
-      LNTH n io_trace = SOME x ⇒
-      ?c s. sem_t (init_st c nd input) t = (Rtimeout, s) ∧
-            n < LENGTH s.io_trace ∧ EL n s.io_trace = x))`;
-
-(* A type soundness proof *)
+(* === A simple type checker and its soundness === *)
 
 val type_permute_pair_lem = Q.prove (
 `!s s1 e1 e2 fst_e snd_e new_nd.
@@ -448,8 +446,9 @@ val type_sound_e = Q.prove (
  rw [] >>
  metis_tac []);
 
-(* Have to use sem_t_ind, and not type_t_ind or t_induction. This is different
- * than small-step-based type soundness *)
+(* Have to use sem_t_ind, and not type_t_ind or t_induction. This is
+   different from small-step-based type soundness *)
+
 val type_sound_t = Q.prove (
 `!s1 t in_for s.
   type_t in_for s t ∧ s ⊆ FDOM s1.store
@@ -525,7 +524,7 @@ val type_sound_t = Q.prove (
          metis_tac [SUBSET_TRANS]) >>
      metis_tac [sem_e_res]));
 
-val type_soundness = Q.prove (
+val type_soundness = Q.store_thm ("type_soundness",
 `!t input. type_t F {} t ⇒ Crash ∉ semantics t input`,
  rw [IN_DEF, semantics_def] >>
  imp_res_tac type_sound_t >>
