examples/fun-op-sem/ml/typeSoundScript.sml
@@ -1,0 +1,1383 @@
+open HolKernel boolLib bossLib lcsymtacs Parse
+     integerTheory stringTheory alistTheory listTheory pred_setTheory
+     pairTheory optionTheory finite_mapTheory arithmeticTheory
+
+(*
+In this file, we demonstrate that the Functional Big-Step semantics
+style is suitable for proofs of type soundness.  In particular, we
+define an ML-like language, heavily inspired by Core ML in Wright and
+Felleisen's "A Syntactic Approach to Type Soundness" (1992) (hereafter
+W&F), using functional big-step semantics rather than small-step
+semantics. We then prove the type soundness using the induction
+theorem generated from the definition of the functional big-step
+semantics.
+*)
+
+(* TODO: from CakeML's miscLib.sml *)
+val _ = set_trace"Goalstack.print_goal_at_top"0
+val SWAP_IMP = PROVE[]``(P ==> Q ==> R) ==> (Q ==> P ==> R)``
+val IMP_IMP = METIS_PROVE[]``(P /\ (Q ==> R)) ==> ((P ==> Q) ==> R)``
+val discharge_hyps = match_mp_tac IMP_IMP >> conj_tac
+fun match_exists_tac tm (g as (_,w)) =
+  let
+    val (vs,b) = strip_exists w
+    val vs = map (fst o dest_var o variant (free_vars tm)) vs
+    fun k (g as (_,w)) =
+      let
+        val (_,b) = strip_exists w
+        val cs = strip_conj b val c = hd cs
+        val (tms,_) = match_term c tm
+        val xs = map #redex tms
+        val ys = map #residue tms
+        fun sorter ls = xs@(List.filter(not o Lib.C Lib.mem xs)ls)
+      in
+        CONV_TAC(RESORT_EXISTS_CONV sorter) >>
+        map_every exists_tac ys
+      end g
+  in
+    CONV_TAC(RENAME_VARS_CONV vs) >> k
+  end g
+(* -- *)
+
+val _ = new_theory"typeSound"
+
+(* TODO: move to HOL standard lib *)
+val LUPDATE_ID = store_thm("LUPDATE_ID",
+  ``∀n ls. n < LENGTH ls ⇒ (LUPDATE (EL n ls) n ls = ls)``,
+  rw[LIST_EQ_REWRITE,EL_LUPDATE] >> rw[])
+(* -- *)
+
+val _ = ParseExtras.temp_tight_equality()
+
+(* Syntax *)
+
+val _ = Datatype`lit =
+  Int int | Unit`
+
+val _ = Datatype`exp =
+  | Lit lit
+  | Var string
+  | App exp exp
+  | Let string exp exp
+  | Fun string exp
+  | Funrec string string exp
+  | Ref exp
+  | Deref exp
+  | Assign exp exp
+  | Letexn string exp
+  | Raise exp exp
+  | Handle exp exp exp`
+
+(* Differences from W&F:
+   - we have specific constants (ints and unit)
+   - we bind one exception at a time
+   - we use Funrec rather than Y
+   - we use explicit syntactic forms for applications of primitives like Ref,
+     Raise, whereas they treat them as curried function values and re-use App to
+     apply them; in our syntax we can of course achieve the same in e by:
+       Let "ref" (Fun "x" (Ref (Var "x"))) e. *)
+
+(*
+The major difference is our separate class of values, which are not in mutual
+recursion with expressions, and include closures. Using closures/environments
+is a stylistic choice that works well with functional big-step and lets us
+avoid defining capture-avoiding substitution over terms (which W&F gloss over
+anyway).
+*)
+
+(* Values *)
+
+val _ = Datatype`v =
+  | Litv lit
+  | Clos ((string,v) alist) string exp
+  | Closrec ((string,v) alist) string string exp
+  | Loc num
+  | Exn num`
+
+val v_induction = theorem"v_induction"
+val v_ind =
+  v_induction
+  |> Q.SPECL[`P`,`EVERY (P o SND)`,`P o SND`]
+  |> SIMP_RULE (srw_ss()) []
+  |> UNDISCH |> CONJUNCT1 |> DISCH_ALL
+  |> GEN_ALL
+  |> curry save_thm "v_ind"
+val v_size_def = definition"v_size_def"
+
+val _ = type_abbrev("env",``:(string,v) alist``)
+
+(* Semantics *)
+
+(*
+The semantics has a state containing the clock, the store, and the number of
+exceptions that have been created.  Whereas W&F's treatment of exceptions is
+intimately tied up with the mechanics of their small-step semantics, we simply
+generate a new exception value for every (dynamic) Letexn expression.
+*)
+
+val _ = Datatype`
+  state = <| clock : num; refs : v list; next_exn : num |>`
+
+val state_component_equality = theorem"state_component_equality"
+
+(* machinery for the functional big-step definition *)
+
+val check_clock_def = Define `
+  check_clock s' s =
+    s' with clock := (if s'.clock ≤ s.clock then s'.clock else s.clock)`;
+
+val check_clock_id = prove(
+  ``!s s'. s.clock ≤ s'.clock ⇒ check_clock s s' = s``,
+ rw [check_clock_def, state_component_equality]);
+
+val dec_clock_def = Define `
+  dec_clock s = s with clock := s.clock - 1`;
+
+val dec_clock_refs = store_thm("dec_clock_refs[simp]",
+  ``(dec_clock s).refs = s.refs``,
+  rw[dec_clock_def])
+
+val dec_clock_next_exn = store_thm("dec_clock_next_exn[simp]",
+  ``(dec_clock s).next_exn = s.next_exn``,
+  rw[dec_clock_def])
+
+val is_closure_def = Define`
+  is_closure (Clos _ _ _) = T ∧
+  is_closure (Closrec _ _ _ _) = T ∧
+  is_closure _ = F`
+val _ = export_rewrites["is_closure_def"]
+
+(* results *)
+
+val _ = Datatype`
+  r = Rval v
+    | Rraise num v
+    | Rfail
+    | Rtimeout`
+
+(* big-step semantics as a function *)
+
+val sem_def = tDefine"sem"`
+  (sem env s (Lit i) = (Rval (Litv i), s)) ∧
+  (sem env s (Var x) =
+    case ALOOKUP env x of
+    | NONE => (Rfail, s)
+    | SOME v => (Rval v, s)) ∧
+  (sem env s (App e1 e2) =
+   case sem env s e1 of
+   | (Rval v1, s1) =>
+       (case sem env (check_clock s1 s) e2 of
+        | (Rval v2, s2) =>
+            if s.clock ≠ 0 ∧ s2.clock ≠ 0 then
+              (case v1 of
+               | Clos env' x e =>
+                 sem ((x,v2)::env') (dec_clock (check_clock s2 s)) e
+               | Closrec env' f x e =>
+                 sem ((x,v2)::(f,v1)::env') (dec_clock (check_clock s2 s)) e
+               | _ => (Rfail, s2))
+            else (Rtimeout, s2)
+        | res => res)
+   | res => res) ∧
+  (sem env s (Let x e1 e2) =
+   case sem env s e1 of
+   | (Rval v1, s1) => sem ((x,v1)::env) (check_clock s1 s) e2
+   | res => res) ∧
+  (sem env s (Fun x e) = (Rval (Clos env x e), s)) ∧
+  (sem env s (Funrec f x e) = (Rval (Closrec env f x e), s)) ∧
+  (sem env s (Ref e) =
+   case sem env s e of
+   | (Rval v, s) => (Rval (Loc (LENGTH s.refs)), s with refs := s.refs ++ [v])
+   | res => res) ∧
+  (sem env s (Deref e) =
+   case sem env s e of
+   | (Rval (Loc n), s) => (if n < LENGTH s.refs then Rval (EL n s.refs) else Rfail, s)
+   | (Rval _, s) => (Rfail, s)
+   | res => res) ∧
+  (sem env s (Assign e1 e2) =
+   case sem env s e1 of
+   | (Rval v1, s1) =>
+     (case sem env (check_clock s1 s) e2 of
+      | (Rval v2, s2) =>
+          (case v1 of
+           | Loc n =>
+             if n < LENGTH s2.refs then
+             (Rval (Litv Unit), s2 with refs := LUPDATE v2 n s2.refs)
+             else (Rfail, s2)
+           | _ => (Rfail, s2))
+      | res => res)
+   | res => res) ∧
+  (sem env s (Letexn x e) =
+   sem ((x,Exn (s.next_exn))::env) (s with next_exn := s.next_exn + 1) e) ∧
+  (sem env s (Raise e1 e2) =
+   case sem env s e1 of
+   | (Rval v1, s1) =>
+     (case sem env (check_clock s1 s) e2 of
+      | (Rval v2, s2) =>
+          (case v1 of
+           | Exn n => (Rraise n v2, s2)
+           | _ => (Rfail, s2))
+      | res => res)
+   | res => res) ∧
+   (sem env s (Handle e3 e1 e2) =
+    case sem env s e1 of
+    | (Rval v1, s1) =>
+      (case v1 of
+       | Exn n =>
+         (case sem env (check_clock s1 s) e2 of
+          | (Rval v2, s2) =>
+            if is_closure v2 then
+              (case sem env (check_clock s2 s) e3 of
+               | (Rraise n3 v3, s3) =>
+                 if n3 = n then
+                   if s.clock ≠ 0 ∧ s3.clock ≠ 0 then
+                     (case v2 of
+                      | Clos env' x e =>
+                        sem ((x,v3)::env') (dec_clock (check_clock s3 s)) e
+                      | Closrec env' f x e =>
+                        sem ((x,v3)::(f,v2)::env') (dec_clock (check_clock s3 s)) e)
+                   else (Rtimeout, s3)
+                 else (Rraise n3 v3, s3)
+               | res => res)
+            else (Rfail, s2)
+          | res => res)
+       | _ => (Rfail, s1))
+    | res => res)`
+(WF_REL_TAC`inv_image (measure I LEX measure exp_size)
+                      (λ(env,s,e). (s.clock,e))` >>
+ rpt strip_tac >> TRY DECIDE_TAC >>
+ fs[check_clock_def,dec_clock_def] >>
+ rw[] >> fsrw_tac[ARITH_ss][])
+
+(*
+clean-up of the definition and induction theorem, removing the check_clock
+machinery that was used to get the function through the termination checker
+*)
+
+val sem_ind = theorem"sem_ind"
+
+val sem_clock = store_thm("sem_clock",
+  ``∀env s e r s'. sem env s e = (r, s') ⇒ s'.clock ≤ s.clock``,
+  ho_match_mp_tac sem_ind >>
+  rpt conj_tac >>
+  simp[sem_def] >>
+  rpt gen_tac >>
+  BasicProvers.EVERY_CASE_TAC >>
+  simp[check_clock_def,dec_clock_def] >>
+  rpt(IF_CASES_TAC >> simp[]) >>
+  rpt strip_tac >> res_tac >> simp[] >> fs[])
+
+val sem_def = store_thm("sem_def",``
+  (sem env s (Lit i) = (Rval (Litv i), s)) ∧
+  (sem env s (Var x) =
+    case ALOOKUP env x of
+    | NONE => (Rfail, s)
+    | SOME v => (Rval v, s)) ∧
+  (sem env s (App e1 e2) =
+   case sem env s e1 of
+   | (Rval v1, s) =>
+       (case sem env s e2 of
+        | (Rval v2, s) =>
+            if s.clock ≠ 0 then
+              (case v1 of
+               | Clos env' x e =>
+                 sem ((x,v2)::env') (dec_clock s) e
+               | Closrec env' f x e =>
+                 sem ((x,v2)::(f,v1)::env') (dec_clock s) e
+               | _ => (Rfail, s))
+            else (Rtimeout, s)
+        | res => res)
+   | res => res) ∧
+  (sem env s (Let x e1 e2) =
+   case sem env s e1 of
+   | (Rval v1, s) => sem ((x,v1)::env) s e2
+   | res => res) ∧
+  (sem env s (Fun x e) = (Rval (Clos env x e), s)) ∧
+  (sem env s (Funrec f x e) = (Rval (Closrec env f x e), s)) ∧
+  (sem env s (Ref e) =
+   case sem env s e of
+   | (Rval v, s) => (Rval (Loc (LENGTH s.refs)), s with refs := s.refs ++ [v])
+   | res => res) ∧
+  (sem env s (Deref e) =
+   case sem env s e of
+   | (Rval (Loc n), s) => (if n < LENGTH s.refs then Rval (EL n s.refs) else Rfail, s)
+   | (Rval _, s) => (Rfail, s)
+   | res => res) ∧
+  (sem env s (Assign e1 e2) =
+   case sem env s e1 of
+   | (Rval v1, s) =>
+     (case sem env s e2 of
+      | (Rval v2, s) =>
+          (case v1 of
+           | Loc n =>
+             if n < LENGTH s.refs then
+             (Rval (Litv Unit), s with refs := LUPDATE v2 n s.refs)
+             else (Rfail, s)
+           | _ => (Rfail, s))
+      | res => res)
+   | res => res) ∧
+  (sem env s (Letexn x e) =
+   sem ((x,Exn (s.next_exn))::env) (s with next_exn := s.next_exn + 1) e) ∧
+  (sem env s (Raise e1 e2) =
+   case sem env s e1 of
+   | (Rval v1, s) =>
+     (case sem env s e2 of
+      | (Rval v2, s) =>
+          (case v1 of
+           | Exn n => (Rraise n v2, s)
+           | _ => (Rfail, s))
+      | res => res)
+   | res => res) ∧
+   (sem env s (Handle e3 e1 e2) =
+    case sem env s e1 of
+    | (Rval v1, s) =>
+      (case v1 of
+       | Exn n =>
+         (case sem env s e2 of
+          | (Rval v2, s) =>
+            if is_closure v2 then
+              (case sem env s e3 of
+               | (Rraise n3 v3, s) =>
+                 if n3 = n then
+                   if s.clock ≠ 0 then
+                     (case v2 of
+                      | Clos env' x e =>
+                        sem ((x,v3)::env') (dec_clock s) e
+                      | Closrec env' f x e =>
+                        sem ((x,v3)::(f,v2)::env') (dec_clock s) e)
+                   else (Rtimeout, s)
+                 else (Rraise n3 v3, s)
+               | res => res)
+            else (Rfail, s)
+          | res => res)
+       | _ => (Rfail, s))
+    | res => res)``,
+  rpt strip_tac >>
+  rw[Once sem_def] >>
+  BasicProvers.CASE_TAC >>
+  imp_res_tac sem_clock >>
+  simp[check_clock_id] >>
+  BasicProvers.CASE_TAC >>
+  imp_res_tac sem_clock >>
+  simp[check_clock_id] >>
+  BasicProvers.EVERY_CASE_TAC >> fs[] >>
+  imp_res_tac sem_clock >>
+  simp[check_clock_id] >>
+  `F` suffices_by rw[] >>
+  DECIDE_TAC)
+
+val sem_ind = store_thm("sem_ind",``
+  ∀P.
+     (∀env s i. P env s (Lit i)) ∧ (∀env s x. P env s (Var x)) ∧
+     (∀env s e1 e2.
+        (∀v3 s1 v1 v4 s2 v2 env' x e.
+           sem env s e1 = (v3,s1) ∧ v3 = Rval v1 ∧
+           sem env s1 e2 = (v4,s2) ∧ v4 = Rval v2 ∧
+           (s2.clock ≠ 0) ∧ v1 = Clos env' x e ⇒
+           P ((x,v2)::env') (dec_clock s2) e) ∧
+        (∀v3 s1 v1 v4 s2 v2 env'' f x' e'.
+           sem env s e1 = (v3,s1) ∧ v3 = Rval v1 ∧
+           sem env s1 e2 = (v4,s2) ∧ v4 = Rval v2 ∧
+           (s2.clock ≠ 0) ∧ v1 = Closrec env'' f x' e' ⇒
+           P ((x',v2)::(f,v1)::env'') (dec_clock s2)
+             e') ∧
+        (∀v3 s1 v1.
+           sem env s e1 = (v3,s1) ∧ v3 = Rval v1 ⇒
+           P env s1 e2) ∧ P env s e1 ⇒
+        P env s (App e1 e2)) ∧
+     (∀env s x e1 e2.
+        (∀v3 s1 v1.
+           sem env s e1 = (v3,s1) ∧ v3 = Rval v1 ⇒
+           P ((x,v1)::env) s1 e2) ∧ P env s e1 ⇒
+        P env s (Let x e1 e2)) ∧ (∀env s x e. P env s (Fun x e)) ∧
+     (∀env s f x e. P env s (Funrec f x e)) ∧
+     (∀env s e. P env s e ⇒ P env s (Ref e)) ∧
+     (∀env s e. P env s e ⇒ P env s (Deref e)) ∧
+     (∀env s e1 e2.
+        (∀v3 s1 v1.
+           sem env s e1 = (v3,s1) ∧ v3 = Rval v1 ⇒
+           P env s1 e2) ∧ P env s e1 ⇒
+        P env s (Assign e1 e2)) ∧
+     (∀env s x e.
+        P ((x,Exn s.next_exn)::env) (s with next_exn := s.next_exn + 1) e ⇒ P env s (Letexn x e)) ∧
+     (∀env s e1 e2.
+        (∀v3 s1 v1.
+           sem env s e1 = (v3,s1) ∧ v3 = Rval v1 ⇒
+           P env s1 e2) ∧ P env s e1 ⇒
+        P env s (Raise e1 e2)) ∧
+     (∀env s e3 e1 e2.
+        (∀v3'' v4' v8 n v3' s2 v2 v4 s3 n3 v3 env' x e.
+           sem env s e1 = (v3'',v4') ∧ v3'' = Rval v8 ∧ v8 = Exn n ∧
+           sem env v4' e2 = (v3',s2) ∧ v3' = Rval v2 ∧
+           is_closure v2 ∧ sem env s2 e3 = (v4,s3) ∧
+           v4 = Rraise n3 v3 ∧ n3 = n ∧ s3.clock ≠ 0 ∧
+           v2 = Clos env' x e ⇒
+           P ((x,v3)::env') (dec_clock s3) e) ∧
+        (∀v3'' v4' v8 n v3' s2 v2 v4 s3 n3 v3 env'' f x' e'.
+           sem env s e1 = (v3'',v4') ∧ v3'' = Rval v8 ∧ v8 = Exn n ∧
+           sem env v4' e2 = (v3',s2) ∧ v3' = Rval v2 ∧
+           is_closure v2 ∧ sem env s2 e3 = (v4,s3) ∧
+           v4 = Rraise n3 v3 ∧ n3 = n ∧ s3.clock ≠ 0 ∧
+           v2 = Closrec env'' f x' e' ⇒
+           P ((x',v3)::(f,v2)::env'') (dec_clock s3)
+             e') ∧
+        (∀v3 v4 v8 n v3' s2 v2.
+           sem env s e1 = (v3,v4) ∧ v3 = Rval v8 ∧ v8 = Exn n ∧
+           sem env v4 e2 = (v3',s2) ∧ v3' = Rval v2 ∧
+           is_closure v2 ⇒
+           P env s2 e3) ∧
+        (∀v3 v4 v8 n.
+           sem env s e1 = (v3,v4) ∧ v3 = Rval v8 ∧ v8 = Exn n ⇒
+           P env v4 e2) ∧ P env s e1 ⇒
+        P env s (Handle e3 e1 e2))
+     ⇒
+     ∀v v1 v2. P v v1 v2``,
+  ntac 2 strip_tac >>
+  ho_match_mp_tac sem_ind >>
+  rw[] >>
+  first_x_assum match_mp_tac >>
+  rw[] >> fs[] >>
+  res_tac >>
+  imp_res_tac sem_clock >>
+  fsrw_tac[ARITH_ss][check_clock_id] >> rfs[] >>
+  fsrw_tac[ARITH_ss][check_clock_id])
+
+(* Typing *)
+
+(*
+Whereas W&F use two categories of type variables (applicative and imperative),
+we follow the more modern approach to making let-polymorphism sound with a
+value restriction.
+*)
+
+val is_value_def = Define`
+  is_value (Lit _) = T ∧
+  is_value (Var _) = T ∧
+  is_value (Fun _ _) = T ∧
+  is_value (Funrec _ _ _) = T ∧
+  is_value _ = F`
+val _ = export_rewrites["is_value_def"]
+
+(* syntax of types *)
+
+val _ = Datatype`tctor =
+  | TC_int
+  | TC_fn
+  | TC_ref
+  | TC_unit
+  | TC_exn`
+
+val _ = Datatype`t =
+  | Tvar string
+  | Tapp (t list) tctor`
+
+val t_size_def = definition"t_size_def"
+val t_induction = theorem"t_induction"
+
+val t_ind =
+  t_induction
+  |> Q.SPECL[`P`,`EVERY P`]
+  |> SIMP_RULE (srw_ss()) []
+  |> UNDISCH |> CONJUNCT1 |> DISCH_ALL
+  |> GEN_ALL
+  |> curry save_thm "t_ind"
+
+val _ = overload_on("Tint",``Tapp [] TC_int``)
+val _ = overload_on("Tfn",``λt1 t2. Tapp [t1;t2] TC_fn``)
+val _ = overload_on("Tref",``λt. Tapp [t] TC_ref``)
+val _ = overload_on("Tunit",``Tapp [] TC_unit``)
+val _ = overload_on("Texn",``λt. Tapp [t] TC_exn``)
+
+(* substitution for variables in a type *)
+
+val tysubst_def = tDefine"tysubst"`
+  (tysubst s (Tvar x) =
+     (case FLOOKUP s x of
+      | SOME t => t
+      | NONE => Tvar x)) ∧
+  tysubst s (Tapp ts tc) =
+    Tapp (MAP (tysubst s) ts) tc`
+(WF_REL_TAC`measure (t_size o SND)` >>
+ rpt gen_tac >> Induct_on`ts` >>
+ rw[t_size_def] >> res_tac >>simp[])
+val tysubst_def =
+  tysubst_def
+  |> SIMP_RULE (std_ss++boolSimps.ETA_ss)[]
+  |> curry save_thm "tysubst_def"
+val _ = export_rewrites["tysubst_def"]
+
+val tysubst_ind = theorem"tysubst_ind"
+
+(* free variables in a type *)
+
+val tyvars_def = tDefine"tyvars"`
+  (tyvars (Tvar x) = {x}) ∧
+  (tyvars (Tapp ts _) = BIGUNION (IMAGE tyvars (set ts)))`
+(WF_REL_TAC`measure (t_size)` >>
+ rpt gen_tac >> Induct_on`ts` >>
+ rw[t_size_def] >> res_tac >>simp[])
+val tyvars_def =
+  tyvars_def
+  |> SIMP_RULE (std_ss++boolSimps.ETA_ss)[]
+  |> curry save_thm "tyvars_def"
+val _ = export_rewrites["tyvars_def"]
+
+(*
+A type environment is a map from (expression) variables to type schemes, where
+a type scheme is a type some of whose variables are considered bound. We
+represent a type scheme by (tvs:string set, t:t), which is t with the variables
+in tvs bound.
+*)
+
+(* free variables in a type environment *)
+
+val tenv_vars_def = Define`
+  tenv_vars tenv =
+    BIGUNION (IMAGE ((λ(tvs,t). tyvars t DIFF tvs) o SND) (set tenv))`
+
+(* typing relation *)
+
+val (type_e_rules,type_e_ind,type_e_cases) = Hol_reln`
+  (type_e tenv (Lit (Int i)) Tint) ∧
+  (type_e tenv (Lit Unit) Tunit) ∧
+  (ALOOKUP tenv x = SOME (tvs,t) ∧ FDOM s ⊆ tvs
+    ⇒ type_e tenv (Var x) (tysubst s t)) ∧
+  (type_e tenv e1 (Tfn t1 t2) ∧
+   type_e tenv e2 t1
+   ⇒ type_e tenv (App e1 e2) t2) ∧
+  (is_value e1 ∧
+   type_e tenv e1 t1 ∧
+   type_e ((x,(tyvars t1 DIFF (tenv_vars tenv),t1))::tenv) e2 t2
+   ⇒ type_e tenv (Let x e1 e2) t2) ∧
+  (¬is_value e1 ∧
+   type_e tenv e1 t1 ∧
+   type_e ((x,({},t1))::tenv) e2 t2
+   ⇒ type_e tenv (Let x e1 e2) t2) ∧
+  (type_e ((x,({},t1))::tenv) e t2
+   ⇒ type_e tenv (Fun x e) (Tfn t1 t2)) ∧
+  (type_e ((x,({},t1))::(f,({},Tfn t1 t2))::tenv) e t2
+   ⇒ type_e tenv (Funrec f x e) (Tfn t1 t2)) ∧
+  (type_e tenv e t ⇒
+   type_e tenv (Ref e) (Tref t)) ∧
+  (type_e tenv e (Tref t) ⇒
+   type_e tenv (Deref e) t) ∧
+  (type_e tenv e1 (Tref t) ∧
+   type_e tenv e2 t ⇒
+   type_e tenv (Assign e1 e2) Tunit) ∧
+  (type_e ((x,({},Texn t1))::tenv) e t2
+   ⇒ type_e tenv (Letexn x e) t2) ∧
+  (type_e tenv e1 (Texn t) ∧
+   type_e tenv e2 t
+   ⇒ type_e tenv (Raise e1 e2) t2) ∧
+  (type_e tenv e3 t3 ∧
+   type_e tenv e1 (Texn t1) ∧
+   type_e tenv e2 (Tfn t1 t3)
+   ⇒ type_e tenv (Handle e3 e1 e2) t3)`
+
+(*
+To state the type soundness theorem, we also need a typing relation on values.
+The typing relation on values has two parameters, rt and et, indicating the
+types of references and exceptions.
+*)
+
+val (type_v_rules,type_v_ind,type_v_cases) = Hol_reln`
+  (type_v rt et (Litv (Int i)) Tint) ∧
+  (type_v rt et (Litv (Unit)) Tunit) ∧
+  (type_env rt et env tenv ∧
+   type_e ((x,({},t1))::tenv) e t2
+   ⇒ type_v rt et (Clos env x e) (Tfn t1 t2)) ∧
+  (type_env rt et env tenv ∧
+   type_e ((x,({},t1))::(f,({},Tfn t1 t2))::tenv) e t2
+   ⇒ type_v rt et (Closrec env f x e) (Tfn t1 t2)) ∧
+  (n < LENGTH rt
+   ⇒ type_v rt et (Loc n) (Tref (EL n rt))) ∧
+  (n < LENGTH et
+   ⇒ type_v rt et (Exn n) (Texn (EL n et))) ∧
+  (type_env rt et [] []) ∧
+  ((∀s. FDOM s ⊆ tvs ⇒ type_v rt et v (tysubst s t)) ∧
+   type_env rt et env tenv
+   ⇒ type_env rt et ((x,v)::env) ((x,(tvs,t))::tenv))`
+
+(* we now have a series of lemmas about the type system *)
+
+val type_e_clauses =
+  [``type_e tenv (Lit i) t``
+  ,``type_e tenv (Var x) t``
+  ,``type_e tenv (App e1 e2) t``
+  ,``type_e tenv (Let x e1 e2) t``
+  ,``type_e tenv (Fun x e) t``
+  ,``type_e tenv (Funrec f x e) t``
+  ,``type_e tenv (Ref e) t``
+  ,``type_e tenv (Deref e) t``
+  ,``type_e tenv (Assign e1 e2) t``
+  ,``type_e tenv (Letexc x e) t``
+  ,``type_e tenv (Raise e1 e2) t``
+  ,``type_e tenv (Handle e3 e1 e2) t``
+  ]
+  |> List.map (SIMP_CONV (srw_ss()) [Once type_e_cases])
+  |> LIST_CONJ
+
+val type_v_clauses =
+  [``type_v s z (Litv i) t``
+  ,``type_v s z (Clos env x e) t``
+  ,``type_v s z (Closrec env f x e) t``
+  ,``type_v s z (Loc n) t``
+  ,``type_v s z (Exn n) t``
+  ]
+  |> List.map (SIMP_CONV (srw_ss()) [Once type_v_cases])
+  |> LIST_CONJ
+
+val type_env_clauses =
+  [``type_env s z [] tenv``
+  ,``type_env s z (x::y) tenv``
+  ]
+  |> List.map (SIMP_CONV (srw_ss()) [Once type_v_cases])
+  |> LIST_CONJ
+
+val type_v_extend = store_thm("type_v_extend",
+  ``(∀v t. type_v s e v t ⇒ type_v (s++s') (e++e') v t) ∧
+    (∀env tenv. type_env s e env tenv ⇒ type_env (s++s') (e++e') env tenv)``,
+  ho_match_mp_tac type_v_ind >>
+  simp[type_v_clauses,type_env_clauses] >>
+  rw[] >> simp[rich_listTheory.EL_APPEND1] >> metis_tac[])
+
+val FINITE_tyvars = store_thm("FINITE_tyvars[simp]",
+  ``∀t. FINITE (tyvars t)``,
+  ho_match_mp_tac t_ind >> simp[] >>
+  simp[EVERY_MEM,PULL_EXISTS])
+
+val tysubst_tysubst = store_thm("tysubst_tysubst",
+  ``∀s t s'. tysubst s' (tysubst s t) = tysubst ((tysubst s' o_f s) ⊌ s') t``,
+  ho_match_mp_tac tysubst_ind >>
+  conj_tac >- (
+    simp[] >>
+    rpt gen_tac >>
+    simp[FLOOKUP_o_f,FLOOKUP_FUNION] >>
+    BasicProvers.CASE_TAC >> simp[] ) >>
+  rw[MAP_MAP_o,MAP_EQ_f])
+
+val tysubst_nil = store_thm("tysubst_nil[simp]",
+  ``∀t. tysubst FEMPTY t = t``,
+  ho_match_mp_tac t_ind >>
+  simp[EVERY_MEM,LIST_EQ_REWRITE,EL_MAP,MEM_EL,PULL_EXISTS])
+
+val tyvars_tysubst = store_thm("tyvars_tysubst",
+  ``∀t. tyvars (tysubst s t) = (tyvars t DIFF FDOM s) ∪ BIGUNION { tyvars u | ∃x. x ∈ tyvars t ∧ FLOOKUP s x = SOME u }``,
+  ho_match_mp_tac t_ind >> simp[] >> rw[] >>
+  TRY BasicProvers.CASE_TAC >>
+  TRY (fs[FLOOKUP_DEF] >> NO_TAC) >> rw[] >- (
+    rw[Once EXTENSION,PULL_EXISTS] ) >>
+  fs[PULL_EXISTS,EVERY_MEM] >>
+  fs[Once EXTENSION,PULL_EXISTS,MEM_MAP] >>
+  metis_tac[])
+
+val tysubst_frees = store_thm("tysubst_frees",
+  ``∀t. (∀x. x ∈ tyvars t ⇒ FLOOKUP s1 x = FLOOKUP s2 x) ⇒
+        tysubst s1 t = tysubst s2 t``,
+  ho_match_mp_tac t_ind >> simp[] >>
+  rw[LIST_EQ_REWRITE,EL_MAP] >>
+  fs[EVERY_MEM,PULL_EXISTS,MEM_EL] >>
+  metis_tac[])
+
+(* alpha-equivalence of type schemes *)
+
+val raconv_def = tDefine"raconv"`
+  (raconv f tvs1 tvs2 (Tvar x1) (Tvar x2) ⇔
+     if x1 ∈ tvs1 then f x1 = x2
+     else x2 = x1 ∧ x1 ∉ tvs2) ∧
+  (raconv f tvs1 tvs2 (Tapp ts1 tc1) (Tapp ts2 tc2) ⇔
+     tc2 = tc1 ∧ LIST_REL (raconv f tvs1 tvs2) ts1 ts2) ∧
+  (raconv _ _ _ _ _ = F)`
+(WF_REL_TAC`measure (t_size o SND o SND o SND o SND)` >>
+ rpt gen_tac >> Induct_on`ts2` >> simp[t_size_def] >>
+ rw[] >> res_tac >> simp[])
+val raconv_def =
+  raconv_def
+  |> SIMP_RULE (std_ss++boolSimps.ETA_ss) []
+  |> curry save_thm "raconv_def"
+val _ = export_rewrites["raconv_def"]
+val raconv_ind = theorem"raconv_ind"
+
+val tsaconv_def = Define`
+  tsaconv (tvs1,t1) (tvs2,t2) ⇔
+    ∃f. BIJ f tvs1 tvs2 ∧
+        raconv f tvs1 tvs2 t1 t2`
+
+val tsaconv_refl = store_thm("tsaconv_refl[simp]",
+  ``∀ts. tsaconv ts ts``,
+  Cases >> simp[tsaconv_def] >>
+  qexists_tac`λx. x` >>
+  conj_tac >- simp[BIJ_ID] >>
+  qid_spec_tac`r` >>
+  ho_match_mp_tac t_ind >>
+  simp[LIST_REL_EL_EQN,EVERY_MEM,MEM_EL,PULL_EXISTS])
+
+val tsaconv_sym = store_thm("tsaconv_sym",
+  ``∀t1 t2. tsaconv t1 t2 ⇒ tsaconv t2 t1``,
+  Cases >> Cases >> simp[tsaconv_def] >>
+  strip_tac >>
+  qexists_tac`LINV f q` >>
+  conj_tac >- simp[BIJ_LINV_BIJ] >>
+  pop_assum mp_tac >>
+  map_every qid_spec_tac[`r'`,`r`] >>
+  ho_match_mp_tac t_ind >>
+  conj_tac >- (
+    gen_tac >> Cases >> simp[] >>
+    `INJ f q q'` by fs[BIJ_DEF] >>
+    rw[] >>
+    imp_res_tac LINV_DEF >>
+    imp_res_tac BIJ_LINV_INV >>
+    metis_tac[INJ_DEF]) >>
+  gen_tac >> strip_tac >>
+  gen_tac >> Cases >> simp[] >>
+  fs[EVERY_MEM,LIST_REL_EL_EQN,MEM_EL,PULL_EXISTS])
+
+val raconv_tyvars_eq = prove(
+  ``∀f tvs1 tvs2 t1 t2.
+      BIJ f tvs1 tvs2 ⇒
+        raconv f tvs1 tvs2 t1 t2 ⇒
+          tyvars t1 DIFF tvs1 =
+          tyvars t2 DIFF tvs2``,
+  ho_match_mp_tac raconv_ind >> reverse(rw[]) >- (
+    fs[Once EXTENSION,PULL_EXISTS] >>
+    fs[LIST_REL_EL_EQN,MEM_EL,PULL_EXISTS] >>
+    metis_tac[] ) >>
+  fs[BIJ_DEF,INJ_DEF] >> metis_tac[] )
+
+val tsaconv_tyvars_eq = store_thm("tsaconv_tyvars_eq",
+  ``∀t1 t2. tsaconv t1 t2 ⇒
+      tyvars (SND t1) DIFF (FST t1) =
+      tyvars (SND t2) DIFF (FST t2)``,
+  Cases >> Cases >> rw[tsaconv_def] >>
+  metis_tac[raconv_tyvars_eq])
+
+val raconv_imp_tysubst = store_thm("raconv_imp_tysubst",
+  ``∀f tvs1 tvs2 t1 t2.
+      FINITE tvs1 ⇒
+      BIJ f tvs1 tvs2 ⇒
+      raconv f tvs1 tvs2 t1 t2 ⇒
+      tysubst (FUN_FMAP (Tvar o f) tvs1) t1 = t2``,
+  ho_match_mp_tac raconv_ind >>
+  rw[] >>
+  simp[FUN_FMAP_DEF,FLOOKUP_FUN_FMAP] >>
+  fs[LIST_REL_EL_EQN,MEM_EL,PULL_EXISTS,LIST_EQ_REWRITE,EL_MAP])
+
+val tsaconv_imp_tysubst = store_thm("tsaconv_imp_tysubst",
+  ``∀t1 t2. tsaconv t1 t2 ⇒
+    FINITE (FST t1) ⇒
+    ∃s. FDOM s = FST t1 ∧
+        FRANGE s = IMAGE Tvar (FST t2) ∧
+        tysubst s (SND t1) = SND t2``,
+  Cases >> Cases >> rw[tsaconv_def] >>
+  imp_res_tac raconv_imp_tysubst >> rw[] >>
+  qexists_tac`FUN_FMAP (Tvar o f) q` >> rw[] >>
+  fs[BIJ_DEF,IMAGE_COMPOSE,IMAGE_SURJ])
+
+val dest_Tvar_def = Define`
+  dest_Tvar (Tvar x) = x`
+val _ = export_rewrites["dest_Tvar_def"]
+
+val tysubst_imp_raconv = store_thm("tysubst_imp_raconv",
+  ``∀f tvs1 tvs2 t1 t2.
+      FINITE tvs1 ∧
+      tysubst (FUN_FMAP (Tvar o f) tvs1) t1 = t2 ∧
+      BIJ f tvs1 tvs2 ∧
+      DISJOINT tvs2 (tyvars t1)
+      ⇒
+      raconv f tvs1 tvs2 t1 t2``,
+  ho_match_mp_tac raconv_ind >> simp[] >>
+  conj_tac >- (
+    rw[] >> rfs[FLOOKUP_DEF,FLOOKUP_FUN_FMAP] ) >>
+  rw[] >> fs[] >- (
+    rw[LIST_REL_EL_EQN,EL_MAP] >>
+    first_x_assum(match_mp_tac o MP_CANON) >>
+    simp[MEM_MAP,PULL_EXISTS] >>
+    qexists_tac`EL n ts1` >>
+    simp[MEM_EL] >>
+    fs[PULL_EXISTS,MEM_EL] >>
+    metis_tac[] ) >>
+  spose_not_then strip_assume_tac >>
+  rfs[FLOOKUP_FUN_FMAP] >>
+  BasicProvers.EVERY_CASE_TAC >> fs[])
+
+val tysubst_imp_aconv = store_thm("tysubst_imp_aconv",
+  ``∀f tvs1 t1 tvs2.
+    FINITE tvs1 ∧
+    BIJ f tvs1 tvs2 ∧
+    DISJOINT tvs2 (tyvars t1)
+    ⇒
+    tsaconv (tvs1,t1) (tvs2,tysubst (FUN_FMAP (Tvar o f) tvs1) t1)``,
+  rw[tsaconv_def] >>
+  qexists_tac`f` >> rw[] >>
+  match_mp_tac tysubst_imp_raconv >>
+  rw[])
+
+val ALOOKUP_MAP_FST_EQ_MAP_SND_REL = store_thm("ALOOKUP_MAP_FST_EQ_MAP_SND_REL",
+  ``∀l1 l2 x y1.
+    MAP FST l1 = MAP FST l2 ∧
+    LIST_REL R (MAP SND l1) (MAP SND l2) ∧
+    ALOOKUP l1 x = SOME y1 ⇒
+    ∃y2. ALOOKUP l2 x = SOME y2 ∧ R y1 y2``,
+  Induct >> simp[] >>
+  Cases >> Cases >> simp[] >>
+  Cases_on`h`>>rw[] >> rw[])
+
+(* the typing rules respect alpha-equivalence *)
+
+val type_e_aconv = store_thm("type_e_aconv",
+  ``∀tenv e t. type_e tenv e t ⇒
+      EVERY (FINITE o FST o SND) tenv ⇒
+      ∀tenv'.
+        MAP FST tenv = MAP FST tenv' ∧
+        LIST_REL tsaconv (MAP SND tenv) (MAP SND tenv') ⇒
+        type_e tenv' e t``,
+  ho_match_mp_tac type_e_ind >>
+  conj_tac >- simp[type_e_clauses] >>
+  conj_tac >- simp[type_e_clauses] >>
+  conj_tac >- (
+    simp[type_e_clauses] >> rw[] >>
+    `∃z. ALOOKUP tenv' x = SOME z ∧ tsaconv (tvs,t) z` by
+      metis_tac[ALOOKUP_MAP_FST_EQ_MAP_SND_REL] >>
+    Cases_on`z`>>simp[]>>
+    first_x_assum(strip_assume_tac o MATCH_MP tsaconv_sym) >>
+    first_assum(mp_tac o MATCH_MP tsaconv_imp_tysubst) >> simp[] >>
+    `FINITE tvs` by (
+      imp_res_tac ALOOKUP_MEM >>
+      fs[EVERY_MEM,FORALL_PROD] >>
+      metis_tac[] ) >>
+    discharge_hyps >- metis_tac[tsaconv_def,FINITE_INJ,BIJ_DEF] >>
+    rw[] >> rw[tysubst_tysubst] >>
+    qexists_tac`tysubst s o_f s'` >> simp[] >>
+    match_mp_tac tysubst_frees >>
+    simp[FLOOKUP_FUNION] >>
+    simp[FLOOKUP_o_f] >>
+    gen_tac >> BasicProvers.CASE_TAC >>
+    strip_tac >>
+    imp_res_tac tsaconv_tyvars_eq >> fs[] >>
+    pop_assum mp_tac >>
+    simp[EXTENSION] >>
+    qmatch_assum_rename_tac`z ∈ tyvars r` >>
+    disch_then(qspec_then`z`mp_tac) >> simp[] >>
+    `z ∉ FDOM s'` by fs[FLOOKUP_DEF] >> simp[] >>
+    simp[tyvars_tysubst] >> strip_tac >>
+    simp[FLOOKUP_DEF] >>
+    fs[SUBSET_DEF] >>
+    metis_tac[] ) >>
+  conj_tac >- (
+    simp[type_e_clauses] >>
+    rw[] >> fs[] >> metis_tac[] ) >>
+  conj_tac >- (
+    simp[type_e_clauses] >> rw[] >> fs[] >>
+    `tenv_vars tenv = tenv_vars tenv'` by (
+      simp[tenv_vars_def,IMAGE_COMPOSE,GSYM LIST_TO_SET_MAP] >>
+      simp[MAP_MAP_o] >>
+      AP_TERM_TAC >> AP_TERM_TAC >>
+      simp[MAP_EQ_f] >>
+      pop_assum mp_tac >>
+      simp[LIST_REL_EL_EQN,LIST_EQ_REWRITE,EL_MAP,GSYM AND_IMP_INTRO] >>
+      rw[] >> res_tac >>
+      imp_res_tac tsaconv_tyvars_eq >>
+      simp[UNCURRY] ) >>
+    qexists_tac`t` >> simp[] >>
+    first_x_assum match_mp_tac >>
+    simp[] ) >>
+  conj_tac >- (
+    simp[type_e_clauses] >> rw[] >> fs[] >>
+    qexists_tac`t` >> simp[] ) >>
+  conj_tac >- ( simp[type_e_clauses] ) >>
+  conj_tac >- ( simp[type_e_clauses] ) >>
+  conj_tac >- ( simp[type_e_clauses] ) >>
+  conj_tac >- ( simp[type_e_clauses] ) >>
+  conj_tac >- (
+    simp[type_e_clauses] >>
+    rw[] >> fs[] >>
+    metis_tac[]) >>
+  conj_tac >- (
+    simp[type_e_clauses] >> rw[] >> fs[] >>
+    `tenv_vars tenv = tenv_vars tenv'` by (
+      simp[tenv_vars_def,IMAGE_COMPOSE,GSYM LIST_TO_SET_MAP] >>
+      simp[MAP_MAP_o] >>
+      AP_TERM_TAC >> AP_TERM_TAC >>
+      simp[MAP_EQ_f] >>
+      pop_assum mp_tac >>
+      simp[LIST_REL_EL_EQN,LIST_EQ_REWRITE,EL_MAP,GSYM AND_IMP_INTRO] >>
+      rw[] >> res_tac >>
+      imp_res_tac tsaconv_tyvars_eq >>
+      simp[UNCURRY] ) >>
+    qexists_tac`t1` >> simp[]) >>
+  conj_tac >- (
+    simp[type_e_clauses] >>
+    rw[] >> fs[] >>
+    metis_tac[]) >>
+  simp[type_e_clauses] >>
+  rw[] >> fs[] >>
+  metis_tac[])
+
+(* a type scheme that is fresh for any finite set of variables exists *)
+
+val fresh_def = new_specification("fresh_def",["fresh"],
+  IN_INFINITE_NOT_FINITE
+  |> Q.ISPECL[`UNIV:string set`,`s:string set`]
+  |> REWRITE_RULE[INST_TYPE[alpha|->``:char``]INFINITE_LIST_UNIV,IN_UNIV]
+  |> SIMP_RULE(srw_ss())[GSYM RIGHT_EXISTS_IMP_THM]
+  |> Q.GEN`s`
+  |> SIMP_RULE(srw_ss())[SKOLEM_THM])
+
+val fresh_seq_def = tDefine"fresh_seq"`
+  fresh_seq avoid n = fresh (avoid ∪ (IMAGE (fresh_seq avoid) (count n)))`
+(WF_REL_TAC`measure (I o SND)` >> simp[])
+val fresh_seq_def =
+  fresh_seq_def
+  |> SIMP_RULE (std_ss++boolSimps.ETA_ss)[]
+  |> curry save_thm "fresh_seq_def"
+
+val fresh_seq_thm = store_thm("fresh_seq_thm",
+  ``∀avoid n.
+      FINITE avoid ⇒
+      fresh_seq avoid n ∉ avoid ∧
+      ∀k. k < n ⇒ fresh_seq avoid n ≠ fresh_seq avoid k``,
+  simp[fresh_seq_def] >>
+  rpt gen_tac >> strip_tac >>
+  Q.PAT_ABBREV_TAC`s = avoid ∪ X` >>
+  `FINITE s` by simp[Abbr`s`] >>
+  qspec_then`s`mp_tac fresh_def >>
+  simp[Abbr`s`] >> rw[] >>
+  fs[fresh_seq_def] >>
+  metis_tac[])
+
+val ALL_DISTINCT_fresh_seq = prove(
+  ``∀n avoid. FINITE avoid ⇒ ALL_DISTINCT (GENLIST (fresh_seq avoid) n)``,
+  Induct >> simp[GENLIST,ALL_DISTINCT_SNOC,MEM_GENLIST] >>
+  metis_tac[fresh_seq_thm])
+
+val DISJOINT_fresh_seq = prove(
+  ``∀n avoid. FINITE avoid ⇒ DISJOINT (set (GENLIST (fresh_seq avoid) n)) avoid``,
+  Induct >> simp[GENLIST,LIST_TO_SET_SNOC] >>
+  metis_tac[fresh_seq_thm])
+
+(* not yet proved (but not yet needed either)
+val fresh_ts_exists = prove(
+  ``∃f. ∀avoid ts.
+      FINITE avoid ∧
+      FINITE (FST ts) ⇒
+      DISJOINT avoid (FST (f avoid ts)) ∧
+      tsaconv ts (f avoid ts)``,
+  simp[GSYM SKOLEM_THM] >>
+  rw[RIGHT_EXISTS_IMP_THM] >>
+  `∃f tvs2. BIJ f (FST ts) tvs2 ∧ DISJOINT tvs2 (tyvars (SND ts) ∪ avoid)` by cheat >>
+  qspecl_then[`f`,`FST ts`,`SND ts`,`tvs2`]mp_tac tysubst_imp_aconv >>
+  simp[] >> fs[] >> simp[Once DISJOINT_SYM] >>
+  strip_tac >>
+  simp[EXISTS_PROD] >>
+  metis_tac[])
+val fresh_ts_def = new_specification("fresh_ts_def",["fresh_ts"],fresh_ts_exists)
+*)
+
+(*
+We have not yet proved the following properties of the type system. The proofs
+will likely require much tedious reasoning about capture-avoiding substitution
+over type schemes. Since they are solely about the type system, and not the
+semantics, this does not depend on whether functional big-step or small-step
+semantics is used. However, these are the only proofs where the value
+restriction is relevant.
+*)
+
+val generalisation_lemma1 = prove(
+  ``type_env rt et env tenv ∧ type_v rt et v t ∧
+    MEM v (MAP SND env) ∧
+    FDOM s ⊆ tyvars t DIFF tenv_vars tenv ⇒
+    type_v rt et v (tysubst s t)``,
+  cheat)
+
+val generalisation_lemma2 = prove(
+  ``type_env rt et env tenv ∧
+    type_env rt et env tenv2 ∧
+    type_e ((x,{},t1)::tenv) e t2 ∧
+    FDOM s ⊆ tyvars (Tfn t1 t2) DIFF tenv_vars tenv2
+    ⇒
+    ∃tenv'.
+      type_env rt et env tenv' ∧
+      type_e ((x,{},tysubst s t1)::tenv') e (tysubst s t2)``,
+  cheat)
+
+val generalisation_lemma3 = prove(
+  ``type_env rt et env tenv ∧
+    type_env rt et env tenv2 ∧
+    type_e ((x,{},t1)::(f,{},Tfn t1 t2)::tenv) e t2 ∧
+    FDOM s ⊆ tyvars (Tfn t1 t2) DIFF tenv_vars tenv2
+    ⇒
+    ∃tenv'.
+      type_env rt et env tenv' ∧
+      type_e ((x,{},tysubst s t1)::(f,{},tysubst s (Tfn t1 t2))::tenv') e (tysubst s t2)``,
+  cheat)
+
+(* lemma about type environment's relationship to value environment *)
+
+val type_env_ALOOKUP_tenv_SOME = prove(
+  ``∀env tenv. type_env rt et env tenv ⇒
+      ∀x tvs t.
+      ALOOKUP tenv x = SOME (tvs,t) ⇒
+      ∃v. ALOOKUP env x = SOME v ∧
+          ∀s. FDOM s ⊆ tvs ⇒
+              type_v rt et v (tysubst s t)``,
+  Induct >> simp[type_env_clauses] >>
+  Cases >> simp[] >>
+  Cases >> simp[] >>
+  PairCases_on`h`>>simp[] >>
+  rw[] >> rw[] >> fs[] >>
+  metis_tac[])
+
+(*
+We prove type soundness by induction on the semantics. This works because both
+the typing relation and the semantics are syntax-directed. We establish that
+well-typed expressions do not fail, if they terminate with a value then the
+value has the same type as the original expression, and if they terminate with
+an exception, the exception's parameter matches the type of the exception.
+*)
+
+val type_soundness = store_thm("type_soundness",
+  ``∀env s e tenv rt et t. type_e tenv e t ⇒
+        LIST_REL (type_v rt et) s.refs rt ⇒
+        type_env rt et env tenv ⇒
+        LENGTH et = s.next_exn ⇒
+        let (r,s') = sem env s e in
+          ∃rt' et'.
+          LIST_REL (type_v (rt++rt') (et++et')) s'.refs (rt++rt') ∧
+          type_env (rt++rt') (et++et') env tenv ∧
+          LENGTH (et++et') = s'.next_exn ∧
+          case r of
+          | Rfail => F
+          | Rval v => type_v (rt++rt') (et++et') v t
+          | Rraise n v =>
+            n < LENGTH (et++et') ∧
+            type_v (rt++rt') (et++et') v (EL n (et++et'))
+          | _ => T``,
+  ho_match_mp_tac sem_ind >>
+  conj_tac >- ( simp[sem_def,type_v_clauses,type_e_clauses,LENGTH_NIL] >> metis_tac[APPEND_NIL]) >>
+  conj_tac >- (
+    rpt gen_tac >>
+    simp[sem_def,type_e_clauses] >>
+    rpt strip_tac >>
+    imp_res_tac type_env_ALOOKUP_tenv_SOME >>
+    simp[] >> rw[LENGTH_NIL] >>
+    qexists_tac`[]`>>rw[]) >>
+  conj_tac >- (
+    rpt gen_tac >>
+    ntac 3 strip_tac >>
+    simp[type_e_clauses,sem_def] >>
+    ntac 6 strip_tac >>
+    `∃r s1. sem env s e = (r,s1)` by metis_tac[pairTheory.PAIR] >> simp[] >>
+    reverse(Cases_on`r`)>>fs[]>-(
+      fs[LET_THM] >> metis_tac[ADD_COMM] ) >- (
+      fs[LET_THM] >> metis_tac[] ) >- (
+      fs[LET_THM] >> metis_tac[ADD_COMM] ) >>
+    `∃r' s2. sem env s1 e' = (r',s2)` by metis_tac[pairTheory.PAIR] >> simp[] >>
+    fs[LET_THM] >>
+    reverse(Cases_on`r'`)>>fs[] >- (
+      first_x_assum(fn th => first_x_assum(mp_tac o MATCH_MP th)) >>
+      disch_then(fn th => first_x_assum(mp_tac o MATCH_MP th)) >>
+      simp[] >> strip_tac >>
+      first_x_assum(fn th => first_x_assum(mp_tac o MATCH_MP th)) >>
+      disch_then(fn th => first_x_assum(mp_tac o MATCH_MP th)) >>
+      discharge_hyps >- metis_tac[type_v_extend] >> strip_tac >>
+      rev_full_simp_tac(srw_ss()++ARITH_ss)[] >>
+      qexists_tac`rt''++rt'''` >>
+      qexists_tac`et''++et'''` >>
+      simp[])
+    >- (
+      first_x_assum(fn th => first_x_assum(mp_tac o MATCH_MP th)) >>
+      disch_then(fn th => first_x_assum(mp_tac o MATCH_MP th)) >>
+      simp[] >> strip_tac >>
+      spose_not_then strip_assume_tac >>
+      first_x_assum(fn th => first_x_assum(mp_tac o MATCH_MP th)) >>
+      disch_then(fn th => first_x_assum(mp_tac o MATCH_MP th)) >>
+      simp[] )
+    >- (
+      first_x_assum(fn th => first_x_assum(mp_tac o MATCH_MP th)) >>
+      disch_then(fn th => first_x_assum(mp_tac o MATCH_MP th)) >>
+      simp[] >> strip_tac >>
+      first_x_assum(fn th => first_x_assum(mp_tac o MATCH_MP th)) >>
+      disch_then(fn th => first_x_assum(mp_tac o MATCH_MP th)) >>
+      simp[] >> strip_tac >>
+      qexists_tac`rt''++rt'''` >>
+      qexists_tac`et''++et'''` >>
+      simp[]) >>
+    reverse IF_CASES_TAC >> simp[] >- (
+      first_x_assum(fn th => first_x_assum(mp_tac o MATCH_MP th)) >>
+      disch_then(fn th => first_x_assum(mp_tac o MATCH_MP th)) >>
+      simp[] >> strip_tac >>
+      first_x_assum(fn th => first_x_assum(mp_tac o MATCH_MP th)) >>
+      disch_then(fn th => first_x_assum(mp_tac o MATCH_MP th)) >>
+      simp[] >> strip_tac >>
+      qexists_tac`rt''++rt'''` >>
+      qexists_tac`et''++et'''` >>
+      simp[]) >>
+    BasicProvers.CASE_TAC >> fs[] >> TRY (
+      fs[type_v_clauses] >> res_tac >> fs[] >> NO_TAC) >>
+    rfs[] >>
+    first_x_assum(fn th => first_x_assum(mp_tac o MATCH_MP th)) >>
+    disch_then(fn th => first_x_assum(mp_tac o MATCH_MP th)) >>
+    simp[] >> strip_tac >>
+    first_x_assum(fn th => first_x_assum(mp_tac o MATCH_MP th)) >>
+    disch_then(fn th => first_x_assum(mp_tac o MATCH_MP th)) >>
+    simp[] >> strip_tac >>
+    fs[type_v_clauses] >>
+    first_x_assum(fn th => first_assum(mp_tac o MATCH_MP th)) >>
+    disch_then(fn th => first_x_assum(mp_tac o MATCH_MP th)) >>
+    simp[type_env_clauses,type_v_clauses,FDOM_EQ_EMPTY] >>
+    (discharge_hyps >- metis_tac[type_v_extend]) >> strip_tac >>
+    fs[UNCURRY] >>
+    BasicProvers.CASE_TAC >> fs[] >>
+    qexists_tac`rt''++rt'''++rt''''` >>
+    qexists_tac`et''++et'''++et''''` >>
+    simp[] >>
+    metis_tac[APPEND_ASSOC,type_v_extend]) >>
+  conj_tac >- (
+    rpt gen_tac >>
+    ntac 2 strip_tac >>
+    simp[type_e_clauses,sem_def] >>
+    `∃r s1. sem env s e = (r,s1)` by metis_tac[pairTheory.PAIR] >> simp[] >>
+    reverse(Cases_on`r`)>>fs[]>-(
+      fs[LET_THM] >> metis_tac[ADD_COMM] ) >- (
+      fs[LET_THM] >> metis_tac[] ) >- (
+      fs[LET_THM] >> metis_tac[ADD_COMM] ) >>
+    `∃r' s2. sem ((x,v)::env) s1 e' = (r',s2)` by metis_tac[pairTheory.PAIR] >> simp[] >>
+    fs[LET_THM] >>
+    rpt gen_tac >> rpt strip_tac >>
+    first_x_assum(fn th => first_x_assum(mp_tac o MATCH_MP th)) >>
+    disch_then(fn th => first_x_assum(mp_tac o MATCH_MP th)) >>
+    simp[] >> strip_tac >>
+    first_x_assum(fn th => first_x_assum(mp_tac o MATCH_MP th)) >>
+    disch_then(fn th => first_x_assum(mp_tac o MATCH_MP th)) >>
+    fs[type_env_clauses,PULL_EXISTS] >> simp[FDOM_EQ_EMPTY] >>
+    TRY(discharge_hyps >- (
+      Cases_on`e`>>fs[sem_def]>>BasicProvers.EVERY_CASE_TAC>>fs[]>>
+      rw[]>>fs[type_v_clauses,LENGTH_NIL]>>rw[]>>fs[]
+      >- (
+        `MEM v (MAP SND env)` by (
+          imp_res_tac ALOOKUP_MEM >>
+          simp[MEM_MAP,EXISTS_PROD] >>
+          metis_tac[] ) >>
+        metis_tac[generalisation_lemma1])
+      >- ( metis_tac[generalisation_lemma2,
+                     SIMP_CONV(srw_ss())[]``tyvars (Tfn t1 t2)``] )
+      >- (
+        match_mp_tac (GEN_ALL(SIMP_RULE(srw_ss())[]generalisation_lemma3))>>
+        metis_tac[]))) >>
+    strip_tac >>
+    BasicProvers.CASE_TAC >> fs[] >>
+    qexists_tac`rt'++rt''` >>
+    qexists_tac`et'++et''` >>
+    simp[]) >>
+  conj_tac >- (
+    simp[type_e_clauses,sem_def,type_v_clauses] >>
+    rw[LENGTH_NIL] >> metis_tac[APPEND_NIL] ) >>
+  conj_tac >- (
+    simp[type_e_clauses,sem_def,type_v_clauses] >>
+    rw[LENGTH_NIL] >> metis_tac[APPEND_NIL]) >>
+  conj_tac >- (
+    simp[type_e_clauses,sem_def,type_v_clauses] >>
+    rw[] >>
+    `∃r s1. sem env s e = (r,s1)` by metis_tac[pairTheory.PAIR] >> simp[] >>
+    reverse(Cases_on`r`)>>fs[]>-(
+      fs[LET_THM] >> metis_tac[] ) >- (
+      fs[LET_THM] >> metis_tac[] ) >- (
+      fs[LET_THM] >> metis_tac[] ) >>
+    simp[type_v_clauses] >>
+    first_x_assum(fn th => first_x_assum(mp_tac o MATCH_MP th)) >>
+    disch_then(fn th => first_x_assum(mp_tac o MATCH_MP th)) >>
+    simp[] >> strip_tac >>
+    qexists_tac`rt''++[t']` >>
+    qexists_tac`et''` >>
+    conj_tac >- (
+      ONCE_REWRITE_TAC[APPEND_ASSOC] >>
+      match_mp_tac rich_listTheory.EVERY2_APPEND_suff >>
+      simp[] >>
+      reverse conj_tac >- metis_tac[type_v_extend,APPEND_NIL] >>
+      match_mp_tac(MP_CANON(GEN_ALL LIST_REL_mono)) >>
+      metis_tac[type_v_extend,APPEND_NIL] ) >>
+    imp_res_tac LIST_REL_LENGTH >>
+    simp[rich_listTheory.EL_APPEND2] >>
+    metis_tac[type_v_extend,APPEND_NIL]) >>
+  conj_tac >- (
+    simp[type_e_clauses,sem_def,type_v_clauses] >>
+    rw[] >>
+    `∃r s1. sem env s e = (r,s1)` by metis_tac[pairTheory.PAIR] >> simp[] >>
+    reverse(Cases_on`r`)>>fs[]>-(
+      fs[LET_THM] >> metis_tac[] ) >- (
+      fs[LET_THM] >> metis_tac[] ) >- (
+      fs[LET_THM] >> metis_tac[] ) >>
+    BasicProvers.CASE_TAC >> fs[] >>
+    TRY(res_tac >> fs[type_v_clauses]>>NO_TAC) >>
+    rw[] >>
+    res_tac >>
+    fs[type_v_clauses] >>
+    fs[LIST_REL_EL_EQN] >>
+    metis_tac[] ) >>
+  conj_tac >- (
+    rpt gen_tac >>
+    ntac 3 strip_tac >>
+    simp[type_e_clauses,sem_def] >>
+    ntac 6 strip_tac >>
+    `∃r s1. sem env s e = (r,s1)` by metis_tac[pairTheory.PAIR] >> simp[] >>
+    reverse(Cases_on`r`)>>fs[]>-(
+      fs[LET_THM] >> metis_tac[ADD_COMM] ) >- (
+      fs[LET_THM] >> metis_tac[] ) >- (
+      fs[LET_THM] >> metis_tac[ADD_COMM] ) >>
+    `∃r' s2. sem env s1 e' = (r',s2)` by metis_tac[pairTheory.PAIR] >> simp[] >>
+    fs[LET_THM] >>
+    reverse(Cases_on`r'`)>>fs[] >- (
+      first_x_assum(fn th => first_x_assum(mp_tac o MATCH_MP th)) >>
+      disch_then(fn th => first_x_assum(mp_tac o MATCH_MP th)) >>
+      simp[] >> strip_tac >>
+      first_x_assum(fn th => first_x_assum(mp_tac o MATCH_MP th)) >>
+      disch_then(fn th => first_x_assum(mp_tac o MATCH_MP th)) >>
+      discharge_hyps >- metis_tac[type_v_extend] >> strip_tac >>
+      metis_tac[APPEND_ASSOC,ADD_ASSOC,ADD_COMM,LENGTH_APPEND] )
+    >- (
+      first_x_assum(fn th => first_x_assum(mp_tac o MATCH_MP th)) >>
+      disch_then(fn th => first_x_assum(mp_tac o MATCH_MP th)) >>
+      simp[] >> strip_tac >>
+      metis_tac[type_v_extend,APPEND_ASSOC,ADD_ASSOC,LENGTH_APPEND,ADD_COMM] )
+    >- (
+      first_x_assum(fn th => first_x_assum(mp_tac o MATCH_MP th)) >>
+      disch_then(fn th => first_x_assum(mp_tac o MATCH_MP th)) >>
+      simp[] >> strip_tac >>
+      first_x_assum(fn th => first_x_assum(mp_tac o MATCH_MP th)) >>
+      disch_then(fn th => first_x_assum(mp_tac o MATCH_MP th)) >>
+      simp[] >> strip_tac >>
+      qexists_tac`rt''++rt'''` >>
+      qexists_tac`et''++et'''` >>
+      simp[]) >>
+    BasicProvers.CASE_TAC >> fs[] >> TRY (
+      fs[type_v_clauses] >> res_tac >> fs[] >> NO_TAC) >>
+    first_x_assum(fn th => first_x_assum(mp_tac o MATCH_MP th)) >>
+    disch_then(fn th => first_x_assum(mp_tac o MATCH_MP th)) >>
+    simp[] >> strip_tac >>
+    first_x_assum(fn th => first_x_assum(mp_tac o MATCH_MP th)) >>
+    disch_then(fn th => first_x_assum(mp_tac o MATCH_MP th)) >>
+    discharge_hyps >- metis_tac[] >> strip_tac >>
+    fs[type_v_clauses] >>
+    rev_full_simp_tac(srw_ss()++ARITH_ss)[] >>
+    reverse IF_CASES_TAC >> fs[type_v_clauses] >- (
+      imp_res_tac LIST_REL_LENGTH >> fs[] >> DECIDE_TAC ) >>
+    Cases_on`n < LENGTH rt` >- (
+      qexists_tac`rt'' ++ rt'''` >>
+      qexists_tac`et'' ++ et'''` >> simp[] >>
+      fs[LIST_REL_EL_EQN,EL_LUPDATE] >> rw[] >>
+      fs[rich_listTheory.EL_APPEND1] ) >>
+    qexists_tac`LUPDATE t' (n-LENGTH rt) (rt'' ++ rt''')` >>
+    qexists_tac`et''++et'''` >>
+    reverse conj_tac >- metis_tac[type_v_extend,LENGTH_APPEND,ADD_ASSOC,ADD_COMM] >>
+    simp[GSYM rich_listTheory.LUPDATE_APPEND2] >>
+    match_mp_tac EVERY2_LUPDATE_same >>
+    simp[rich_listTheory.EL_APPEND1,rich_listTheory.EL_APPEND2] >>
+    simp[rich_listTheory.LUPDATE_APPEND1,rich_listTheory.LUPDATE_APPEND2] >>
+    simp[LUPDATE_ID] >> rw[] >>
+    qpat_assum`type_v A X Y Z`mp_tac >>
+    simp[rich_listTheory.EL_APPEND2]) >>
+  conj_tac >- (
+    rpt gen_tac >>
+    strip_tac >>
+    simp[type_e_clauses,sem_def] >>
+    rpt gen_tac >> rpt strip_tac >>
+    Q.PAT_ABBREV_TAC`env' =X::env` >>
+    Q.PAT_ABBREV_TAC`s' = s with next_exn := Y` >>
+    `∃r s1. sem env' s' e = (r,s1)` by metis_tac[pairTheory.PAIR] >> simp[] >>
+    fs[LET_THM,Abbr`s'`,Abbr`env'`,type_env_clauses,PULL_EXISTS,type_v_clauses] >>
+    first_x_assum(fn th => first_x_assum(mp_tac o MATCH_MP th)) >>
+    disch_then(qspecl_then[`rt`,`et++[t1]`]mp_tac) >>
+    discharge_hyps >- (
+      match_mp_tac(MP_CANON(GEN_ALL LIST_REL_mono)) >>
+      metis_tac[type_v_extend,APPEND_NIL] ) >>
+    simp[rich_listTheory.EL_APPEND2,FDOM_EQ_EMPTY] >>
+    discharge_hyps >- metis_tac[type_v_extend,APPEND_NIL] >>
+    strip_tac >>
+    qexists_tac`rt''` >>
+    qexists_tac`[t1]++et''` >>
+    simp[] >>
+    Cases_on`r`>>fs[]>>
+    simp[]) >>
+  conj_tac >- (
+    rpt gen_tac >>
+    ntac 2 strip_tac >>
+    simp[type_e_clauses,sem_def] >>
+    rpt strip_tac >>
+    `∃r s1. sem env s e = (r,s1)` by metis_tac[pairTheory.PAIR] >> simp[] >>
+    (Cases_on`r`)>>fs[LET_THM]>>TRY(metis_tac[ADD_COMM])>>
+    `∃r s2. sem env s1 e' = (r,s2)` by metis_tac[pairTheory.PAIR] >> simp[] >>
+    first_x_assum(fn th => first_x_assum(mp_tac o MATCH_MP th)) >>
+    disch_then(fn th => first_x_assum(mp_tac o MATCH_MP th)) >>
+    simp[] >> strip_tac>>
+    first_x_assum(fn th => first_x_assum(mp_tac o MATCH_MP th)) >>
+    disch_then(fn th => first_x_assum(mp_tac o MATCH_MP th)) >>
+    discharge_hyps >- metis_tac[] >> strip_tac >> rfs[] >>
+    rev_full_simp_tac(srw_ss()++ARITH_ss)[] >>
+    reverse(Cases_on`r`)>>fs[LET_THM]
+    >-(metis_tac[APPEND_ASSOC,LENGTH_APPEND,ADD_ASSOC,ADD_COMM])
+    >-(qexists_tac`rt''++rt'''`>>
+       qexists_tac`et''++et'''`>>
+       simp[] ) >>
+    Cases_on`v`>>fs[type_v_clauses]>>
+    qexists_tac`rt''++rt'''`>>
+    qexists_tac`et''++et'''`>>
+    simp[] >> simp[rich_listTheory.EL_APPEND1] >>
+    metis_tac[] ) >>
+  rpt gen_tac >>
+  ntac 3 strip_tac >>
+  simp[type_e_clauses,sem_def] >>
+  rpt strip_tac >>
+  `∃r s1. sem env s e' = (r,s1)` by metis_tac[pairTheory.PAIR] >> simp[] >>
+  (Cases_on`r`)>>fs[LET_THM]>>TRY(metis_tac[ADD_COMM])>>
+  `∃r s2. sem env s1 e'' = (r,s2)` by metis_tac[pairTheory.PAIR] >> simp[] >>
+  first_x_assum(fn th => first_x_assum(mp_tac o MATCH_MP th)) >>
+  disch_then(fn th => first_x_assum(mp_tac o MATCH_MP th)) >>
+  simp[] >> strip_tac>>
+  Cases_on`v`>>TRY(fs[type_v_clauses]>>NO_TAC)>>simp[]>> fs[] >>
+  first_x_assum(fn th => first_x_assum(mp_tac o MATCH_MP th)) >>
+  disch_then(fn th => first_x_assum(mp_tac o MATCH_MP th)) >>
+  discharge_hyps >- metis_tac[] >> strip_tac >> rfs[] >>
+  rev_full_simp_tac(srw_ss()++ARITH_ss)[] >>
+  reverse(Cases_on`r`)>>fs[LET_THM]
+  >-(qexists_tac`rt''++rt'''`>>
+     qexists_tac`et''++et'''`>>
+     simp[] )
+  >-(qexists_tac`rt''++rt'''`>>
+     qexists_tac`et''++et'''`>>
+     simp[] ) >>
+  `∃r s3. sem env s2 e = (r,s3)` by metis_tac[pairTheory.PAIR] >> simp[] >>
+  reverse IF_CASES_TAC >> fs[] >- (
+    Cases_on`v`>>fs[type_v_clauses] ) >>
+  first_x_assum(fn th => first_x_assum(mp_tac o MATCH_MP th)) >>
+  disch_then(fn th => first_x_assum(mp_tac o MATCH_MP th)) >>
+  discharge_hyps >- metis_tac[] >> strip_tac >> rfs[] >>
+  rev_full_simp_tac(srw_ss()++ARITH_ss)[] >>
+  reverse(Cases_on`r`)>>fs[LET_THM]
+  >-(qexists_tac`rt''++rt'''++rt''''`>>
+     qexists_tac`et''++et'''++et''''`>>
+     simp[] )
+  >-(
+    reverse IF_CASES_TAC >> fs[] >-(qexists_tac`rt''++rt'''++rt''''`>>
+                                    qexists_tac`et''++et'''++et''''`>>
+                                    simp[] ) >>
+    reverse IF_CASES_TAC >> fs[] >-(qexists_tac`rt''++rt'''++rt''''`>>
+                                    qexists_tac`et''++et'''++et''''`>>
+                                    simp[] ) >>
+    Cases_on`v`>>fs[type_v_clauses] >>
+    first_x_assum(fn th => first_assum(mp_tac o MATCH_MP th)) >>
+    disch_then(fn th => first_x_assum(mp_tac o MATCH_MP th)) >>
+    simp[type_env_clauses,FDOM_EQ_EMPTY] >>
+    (discharge_hyps >- (
+       rev_full_simp_tac(srw_ss()++ARITH_ss)[rich_listTheory.EL_APPEND1] >>
+       simp[type_v_clauses] >>
+       metis_tac[type_v_extend,APPEND_ASSOC] ) ) >>
+    simp[UNCURRY] >> strip_tac >>
+    BasicProvers.CASE_TAC >> fs[] >>
+    qexists_tac`rt''++rt'''++rt''''++rt'''''`>>
+    qexists_tac`et''++et'''++et''''++et'''''`>>
+    simp[] >>
+    metis_tac[type_v_extend,APPEND_ASSOC] )
+  >-(qexists_tac`rt''++rt'''++rt''''`>>
+     qexists_tac`et''++et'''++et''''`>>
+     simp[] ))
+
+val _ = export_theory()
